src/goose_lang/proofmode.v
@@ -3,7 +3,7 @@ From iris.proofmode Require Export environments.
 From Perennial.Helpers Require Export ipm.
 From Perennial.program_logic Require Export weakestpre.
 From Perennial.goose_lang Require Export lang lifting.
-From Perennial.goose_lang Require Export typing new.exception.
+From Perennial.goose_lang Require Export typing new.exception new.loop.impl.
 Set Default Proof Using "Type".
 Import uPred.
 
@@ -200,7 +200,9 @@ Ltac wp_pure_filter e' :=
   first [ lazymatch e' with (App (Val (RecV _ _ _)) (Val _)) => idtac end
         | eunify e' (do: (Val _))%E
         | eunify e' (return: (Val _))%E
-        | eunify e' (exception_seq (Val _) (Val _))%E
+        | eunify e' (continue: (Val _))%E
+        | eunify e' (break: (Val _))%E
+        | eunify e' (exception_seq _ (Val _))%E
         | eunify e' (App exception_do (Val _))%E
         | eunify e' (rec: _ _ := _)%E
         | eunify e' (InjL (Val _))
